coq/alternative/Machine.v
@@ -1,0 +1,41 @@
+Require Import Coq.Lists.List.
+
+Record Machine :=
+  mkMachine
+    { S : Type;
+      Σ : Type;
+      Λ : Type;
+      S0 : S;
+      δ : S -> Σ -> S;
+      ω : S -> Σ -> list Λ
+    }.
+
+Section MachineSemantics.
+  Variable M : Machine.
+
+  Record Configuration : Type :=
+    mkConfiguration {
+        source : S M;
+        input : Σ M;
+        destination : S M;
+        output : list (Λ M);
+      }.
+
+  Inductive Trace : list Configuration -> Prop :=
+  | Trace_start : forall σ,
+      Trace (mkConfiguration (S0 M) σ (δ M (S0 M) σ) (ω M (S0 M) σ)
+               ::nil)
+  | Trace_next : forall ts src σ s' σ' λs',
+      Trace (mkConfiguration s' σ' src λs'
+               ::ts) ->
+      Trace (mkConfiguration src σ (δ M src σ) (ω M src σ)
+               ::mkConfiguration s' σ' src λs'
+               ::ts).
+
+  Definition Semantics
+             (σs : list (Σ M))
+             (λs : list (list (Λ M))) : Prop :=
+    forall ts, Trace ts ->
+               σs = List.map input ts /\
+               λs = List.map output ts.
+End MachineSemantics.
