coq/alternative/TypingFacts.v
@@ -1,0 +1,155 @@
+Require Import Coq.Strings.String.
+Require Import Coq.Vectors.Vector.
+Require Import Coq.Sets.Ensembles.
+Require Import SMEDL.Types.
+Require Import SMEDL.AST.
+Require SMEDL.VarEnv.
+Import SMEDL.VarEnv.Notations.
+Import SMEDL.VarEnv.Coercions.
+Require SMEDL.EventEnv.
+Import SMEDL.EventEnv.Notations.
+Import SMEDL.EventEnv.Coercions.
+
+Require Import SMEDL.Typing.
+
+Arguments exist {_ _} _ _.
+Arguments existT {_ _} _ _.
+
+(* Equivalence of event environments relies on Ensemble extensionality and
+ Functional Extensionality. Is that OK?*)
+
+Require Import Coq.Logic.FunctionalExtensionality.
+
+(* The event declarations completely determine the event type environment, when
+one exists. *)
+Lemma HasTy_EventEnv_unique : forall es Δ1 Δ2,
+    HasTy_EventEnv es Δ1 ->
+    HasTy_EventEnv es Δ2 ->
+    Δ1 = Δ2.                  (* TODO: = or some other equivalence? *)
+Proof.
+  intros.
+  inversion H; inversion H0.
+  destruct Δ1, Δ2.
+  simpl in *.
+
+  assert (Heq : events0 = events)
+    by (apply Extensionality_Ensembles;
+        unfold Same_set, Included;
+        firstorder).
+  subst.
+
+  assert (Heq : arity0 = arity).
+  { extensionality x.
+    specialize (H10 x).
+    specialize (H4 x).
+    destruct x.
+    specialize (H7 x).
+    inversion H7.
+    specialize (H14 i).
+    inversion H14.
+    specialize (H10 x0).
+    specialize (H4 x0).
+    rewrite <- H10, <- H4;
+      simpl; auto.
+  }
+  subst.
+
+  assert (Heq : param_name0 = param_name).
+  { extensionality x.
+    apply Vector.eq_nth_iff; intros; subst.
+    specialize (H5 x).
+    specialize (H11 x).
+    destruct x.
+    specialize (H7 x).
+    inversion H7.
+    specialize (H14 i).
+    inversion H14.
+    specialize (H5 x0).
+    specialize (H11 x0).
+    simpl in *.
+    specialize (H5 H15 p2).
+    specialize (H11 H15 p2).
+    rewrite H5 in H11.
+    inversion H11.
+    rewrite H17.
+    auto.
+  }
+  subst.
+
+  assert (Heq : lookup0 = lookup).
+  { extensionality x.
+    apply Vector.eq_nth_iff; intros; subst.
+    specialize (H6 x).
+    specialize (H12 x).
+    destruct x.
+    specialize (H7 x).
+    inversion H7.
+    specialize (H14 i).
+    inversion H14.
+    specialize (H6 x0).
+    specialize (H12 x0).
+    simpl in *.
+    specialize (H6 H15 p2).
+    specialize (H12 H15 p2).
+    rewrite H6 in H12.
+    inversion H12.
+    rewrite H17.
+    auto.
+  }
+  subst.
+
+  assert (Heq : param_names_unique0 = param_names_unique).
+  { extensionality x.
+    extensionality n1.
+    extensionality n2.
+    extensionality Hn1n2.
+    Require Import Eqdep_dec.
+    apply eq_proofs_unicity.
+    clear.
+    intros.
+    destruct (Fin.eq_dec x0 y); intuition.
+  }
+  subst.
+
+  reflexivity.
+Qed.
+
+(* The global variable declarations completely determine the global variable
+environment, when one exist. *)
+Lemma HasTy_Var_unique : forall gs Γ1 Γ2,
+    HasTy_VarEnv gs Γ1 ->
+    HasTy_VarEnv gs Γ2 ->
+    Γ1 = Γ2.                  (* TODO: = or some other equivalence? *)
+Proof.
+  intros.
+  inversion H; inversion H0.
+  destruct Γ1, Γ2; simpl in *.
+
+  assert (vars0 = vars)
+    by (apply Extensionality_Ensembles;
+        unfold Same_set, Included;
+        firstorder).
+  subst.
+
+  assert (lookup = lookup0).
+  { extensionality v.
+    specialize (H3 v).
+    specialize (H6 v).
+    destruct v.
+    specialize (H2 x).
+    inversion H2.
+    specialize (H7 i).
+    inversion H7 as [ty Hty].
+    specialize (H3 ty).
+    specialize (H6 ty).
+    inversion H3.
+    inversion H6.
+    specialize (H10 Hty).
+    specialize (H12 Hty).
+    rewrite H10.
+    rewrite H12.
+    reflexivity.
+  }
+  subst.
+  reflexivity.
+Qed.
